\documentclass{article}
\usepackage{graphicx} % Required for inserting images
\usepackage{amsmath}
\usepackage{amsthm}
\usepackage{amssymb}
\usepackage{xcolor}


\setlength{\topmargin}{-.5in}
\setlength{\oddsidemargin}{0 in}
\setlength{\evensidemargin}{0 in}
\setlength{\textwidth}{6.5truein}
\setlength{\textheight}{8.5truein}

\renewcommand\qedsymbol{$\blacksquare$}

\begin{document}
    \begin{proof}
        \[
            C(t) = (1 - t)^3b_0 + 3(1 - t)^2tb_1 + 3(1 - t)t^2b_2 + t^3b_3
            \]
            \begin{align*}
                C'(t) & = 3(1 - t)^2(-1)b_0 + 3(2(1 - t)(-1)t + (1 - t)^2)b_1 + 3((-1)t^2 + 2(1 - t)t)b_2 + 3t^2b_3
                \\ & =
                -3(1 - t)^2b_0 + 3(-2(1 - t)t + (1 - t)^2)b_1 + 3(-t^2 + 2(1 - t)t)b_2 + 3t^2b_3
                \\ & =
                -3(1 - t)^2b_0 - 6(1 - t)tb_1 + 3(1 - t)^2b_1 - 3t^2b_2 + 6(1 - t)tb_2 + 3t^2b_3
            \end{align*}
            \begin{align*}
                C''(t) & = -3(2(1 - t)(-1))b_0 - 6((1-t) + (-1)t)b_1 + 3(2(1 - t)(-1))b_1 - 6tb_2 +6((-1)t + (1 - t))b_2 + 6tb_3
                \\ & =
                6(1 - t)b_0 - 6(1 - t)b_1 + 6tb_1 - 6(1 - t)b_1 - 6tb_2 - 6tb_2 + 6(1 - t)b_2 + 6tb_3
                \\ & =
                6b_0 - 6tb_0 - 6b_1 + 6tb_1 + 6tb_1 - 6b_1 + 6tb_1 - 12tb_2 + 6b_2 - 6tb_2 + 6tb_3
                \\ & =
                6b_0 - 6tb_0 - 12b_1 + 18tb_1 - 18tb_2 + 6b_2 + 6tb_3
            \end{align*}
            Now, since $C(0) = b_0$ the second derivative at $b_0$ is
            \begin{align*}
                C''(0) & = 6b_0 - 6(0)b_0 - 12b_1 + 18(0)b_1 - 18(0)b_2 + 6b_2 + 6(0)b_3
                \\ & =
                6b_0 - 12b_1 + 6b_2
                \\ & =
                6(b_0 - 2b_1 + b_2)
            \end{align*}
            as desired, and since $C(1) = b_3$, the second derivative at $b_3$ is
            \begin{align*}
                C''(1) & = 6b_0 - 6(1)b_0 - 12b_1 + 18(1)b_1 - 18(1)b_2 + 6b_2 + 6(1)b_3
                \\ & =
                6b_0 - 6b_0 - 12b_1 + 18b_1 - 18b_2 + 6b_2 + 6b_3
                \\ & =
                0 + 6b_1 - 12b_2 + 6b_3
                \\ & =
                6(b_1 - 2b_2 + b_3)
            \end{align*}
            as desired
    \end{proof}
\end{document}
